WIP

src/lcertify/Certify.v
@@ -137,16 +137,387 @@ Inductive sim_lc (tid:Id.t) (ts:Time.t) (lc1 lc2:Local.t (A:=unit)) (mem1 mem2:M
     (FWDBANK: forall loc,
         opt_rel
           (fun fwd1 fwd2 =>
-             fwd2.(FwdItem.ts) <= ts ->
-             (fwd1.(FwdItem.ts) = fwd2.(FwdItem.ts) /\
-              sim_view ts fwd1.(FwdItem.view) fwd2.(FwdItem.view) /\
-              fwd1.(FwdItem.ex) = fwd2.(FwdItem.ex)))
+             fwd2.(FwdItem.view).(View.ts) <= ts ->
+             Memory.read loc fwd1.(FwdItem.ts) mem1 = Memory.read loc fwd2.(FwdItem.ts) mem2 /\
+             sim_view ts fwd1.(FwdItem.view) fwd2.(FwdItem.view) /\
+             fwd1.(FwdItem.ex) = fwd2.(FwdItem.ex))
           (lc1.(Local.fwdbank) loc) (lc2.(Local.fwdbank) loc))
     (EXBANK: opt_rel (sim_exbank tid ts mem1 mem2) lc1.(Local.exbank) lc2.(Local.exbank))
     (PROMISES: lc1.(Local.promises) = lc2.(Local.promises))
-    (PROMISES_TS: forall mid (FIND: Promises.lookup mid lc1.(Local.promises)), mid <= ts)
+    (PROMISES_TS: forall mid (FIND: Promises.lookup mid lc2.(Local.promises)), mid <= ts)
 .
 Hint Constructors sim_lc.
+
+Inductive sim_mem (tid:Id.t) (ts:Time.t) (mem1 mem2:Memory.t): Prop :=
+| sim_mem_intro
+    (EQUIV: forall tsx (TSX: tsx <= ts), Memory.get_msg tsx mem1 = Memory.get_msg tsx mem2)
+.
+Hint Constructors sim_mem.
+
+Inductive sim_eu (tid:Id.t) (ts:Time.t) (eu1 eu2:ExecUnit.t (A:=unit)): Prop :=
+| sim_eu_intro
+    (STATE: sim_state ts eu1.(ExecUnit.state) eu2.(ExecUnit.state))
+    (LOCAL: sim_lc tid ts eu1.(ExecUnit.local) eu2.(ExecUnit.local) eu1.(ExecUnit.mem) eu2.(ExecUnit.mem))
+    (MEM: sim_mem tid ts eu1.(ExecUnit.mem) eu2.(ExecUnit.mem))
+.
+Hint Constructors sim_eu.
+
+Lemma sim_time_join
+      ts l1 l2 r1 r2
+      (VIEW1: sim_time ts l1 r1)
+      (VIEW2: sim_time ts l2 r2):
+  sim_time ts (join l1 l2) (join r1 r2).
+Proof.
+  inv VIEW1. inv VIEW2.
+  econs. intro X. unfold join, Time.join in X. apply Time.max_lub_iff in X. des.
+  eauto.
+Qed.
+
+Lemma sim_val_const
+      ts c:
+  sim_val ts (ValA.mk _ c bot) (ValA.mk _ c bot).
+Proof.
+  econs. ss.
+Qed.
+
+Lemma sim_view_bot
+      ts:
+  sim_view ts bot bot.
+Proof.
+  econs. ss.
+Qed.
+
+Lemma sim_view_const
+      ts c:
+  sim_view ts (View.mk c bot) (View.mk c bot).
+Proof.
+  econs. ss.
+Qed.
+
+Lemma sim_view_join
+      ts l1 l2 r1 r2
+      (VIEW1: sim_view ts l1 r1)
+      (VIEW2: sim_view ts l2 r2):
+  sim_view ts (join l1 l2) (join r1 r2).
+Proof.
+  destruct l1 as [lt1 lv1].
+  destruct l2 as [lt2 lv2].
+  destruct r1 as [rt1 rv1].
+  destruct r2 as [rt2 rv2].
+  inv VIEW1. inv VIEW2. ss.
+  econs. s. intro X. unfold join, Time.join in X. apply Time.max_lub_iff in X. des.
+  specialize (TS X). specialize (TS0 X0). des. inv TS. inv TS0. ss.
+Qed.
+
+Lemma sim_view_ifc
+      ts c l1 r1
+      (VIEW1: sim_view ts l1 r1):
+  sim_view ts (ifc c l1) (ifc c r1).
+Proof.
+  destruct c; ss.
+Qed.
+
+Lemma sim_val_view ts v1 v2
+      (VAL: sim_val ts v1 v2):
+  sim_view ts v1.(ValA.annot) v2.(ValA.annot).
+Proof.
+  inv VAL. econs. i. specialize (TS H). des. subst. ss.
+Qed.
+
+Lemma sim_rmap_expr
+      ts rmap1 rmap2 e
+      (RMAP: sim_rmap ts rmap1 rmap2):
+  sim_val ts (sem_expr rmap1 e) (sem_expr rmap2 e).
+Proof.
+  induction e; s.
+  - apply sim_val_const.
+  - unfold RMap.find. inv RMAP. specialize (RMAP0 reg). inv RMAP0; ss.
+  - econs. s. i. inv IHe. specialize (TS H). des. congr.
+  - econs. s. i. unfold join, Time.join in H. apply Time.max_lub_iff in H. des.
+    inv IHe1. inv IHe2.
+    specialize (TS H). specialize (TS0 H0). des. congr.
+Qed.
+
+Lemma sim_rmap_add
+      ts rmap1 rmap2 v1 v2 r
+      (RMAP: sim_rmap ts rmap1 rmap2)
+      (VAL: sim_val ts v1 v2):
+  sim_rmap ts (RMap.add r v1 rmap1) (RMap.add r v2 rmap2).
+Proof.
+  inv RMAP. econs. ii. unfold RMap.add. rewrite ? IdMap.add_spec.
+  condtac; ss. inversion e. subst. econs. ss.
+Qed.
+
+(* TODO: move *)
+Lemma internal_bot_inv
+      A `{orderC A eq}
+      lc1 lc2
+      (LC: Local.internal (A:=A) bot lc1 lc2):
+  lc2 = lc1.
+Proof.
+  inv LC. destruct lc1. s. f_equal.
+  rewrite bot_join; ss. apply View.order.
+Qed.
+
+Lemma sim_eu_step
+      tid ts eu1 eu2 eu2'
+      (SIM: sim_eu tid ts eu1 eu2)
+      (STEP: certify_step tid eu2 eu2')
+      (WF1: ExecUnit.wf tid eu1)
+      (WF2: ExecUnit.wf tid eu2):
+      (* TODO: remove *)
+      (* (VWP: eu2'.(ExecUnit.local).(Local.vwp).(View.ts) <= ts) *)
+      (* (VCAP: eu2'.(ExecUnit.local).(Local.vcap).(View.ts) <= ts): *)
+  exists eu1',
+    <<STEP: certify_step tid eu1 eu1'>> /\
+    <<SIM: sim_eu tid ts eu1' eu2'>>.
+Proof.
+  exploit certify_step_wf; eauto. i.
+  destruct eu1 as [[stmts1 rmap1] lc1 mem1].
+  destruct eu2 as [[stmts2 rmap2] lc2 mem2].
+  destruct eu2' as [[stmts2' rmap2'] lc2' mem2'].
+  inv SIM. inv STATE. ss. subst. inv STEP; cycle 1.
+  { (* write step *)
+    admit.
+  }
+  { (* state step *)
+    inv STEP0. inv STEP. ss. subst. inv STATE; inv LOCAL0; inv EVENT.
+    - (* skip *)
+      apply internal_bot_inv in LC. subst.
+      eexists (ExecUnit.mk _ _ _). esplits.
+      + econs 1. econs. econs; ss; cycle 1.
+        * econs 1; eauto. econs; eauto.
+        * s. econs 1.
+      + econs; ss. econs; ss; try by apply LOCAL.
+        rewrite bot_join; [|by apply View.order]. apply LOCAL.
+    - (* assign *)
+      apply internal_bot_inv in LC. subst.
+      eexists (ExecUnit.mk _ _ _). esplits.
+      + econs 1. econs. econs; ss; cycle 1.
+        * econs 1; eauto. econs; eauto.
+        * s. econs 2. ss.
+      + econs; ss. econs; ss; try by apply LOCAL.
+        * apply sim_rmap_add; ss. apply sim_rmap_expr. ss.
+        * rewrite bot_join; [|by apply View.order]. destruct lc1. ss.
+    - (* read *)
+
+
+
+              (* TODO: move *)
+              Lemma sim_view_eq
+                    ts v1 v2
+                    (SIM: sim_view ts v1 v2)
+                    (V2: v2.(View.ts) <= ts):
+                v1 = v2.
+              Proof.
+                apply SIM. ss.
+              Qed.
+              Lemma sim_time_eq
+                    ts v1 v2
+                    (SIM: sim_time ts v1 v2)
+                    (V2: v2 <= ts):
+                v1 = v2.
+              Proof.
+                apply SIM. ss.
+              Qed.
+
+              
+      inv STEP.
+      match goal with
+      | [|- context[join (joins ?l) ?f]] =>
+        remember (join (joins l) f) as post eqn:POST
+      end.
+      destruct (le_dec post.(View.ts) ts).
+      { (* read's post-view <= ts. *)
+        rename l into TS0.
+        exploit sim_rmap_expr; eauto. i. inv x1. exploit TS.
+        { rewrite <- TS0. s. rewrite <- join_l, <- join_l. eauto. }
+        intro ELOC. clear TS.
+        
+
+
+        eexists (ExecUnit.mk _ _ _). esplits.
+        + econs 1. econs. econs; ss; cycle 1.
+          * econs 2; eauto. econs.
+            4: instantiate (1 :=
+                              match Local.fwdbank lc2 (ValA.val (sem_expr rmap2 eloc)) with
+                              | Some fwd => 
+                              ts0).
+            1: instantiate (1 := (sem_expr rmap1 eloc)).
+            all: ss.
+            { rewrite ELOC. exploit sim_time_eq.
+              { inv LOCAL. eapply COH0. }
+              { rewrite <- TS0. admit. }
+              intro COH'. rewrite COH'. ss.
+            }
+            { admit. (* latest *) }
+            {
+              (* TODO: move *)
+              Lemma sim_mem_read
+                    tid ts mem1 mem2 loc ts0
+                    (SIM: sim_mem tid ts mem1 mem2)
+                    (TS0: ts0 <= ts):
+                Memory.read loc ts0 mem1 = Memory.read loc ts0 mem2.
+              Proof.
+                inv SIM. generalize (EQUIV _ TS0). unfold Memory.get_msg, Memory.read. destruct ts0; ss.
+                intro X. rewrite X. ss.
+              Qed.
+
+              rewrite ELOC,  <- MSG. revert TS0.
+              destruct (Local.fwdbank lc2 (ValA.val (sem_expr rmap2 eloc))) as [[]|] eqn:FWD; cycle 1.
+              { i. eapply sim_mem_read; eauto. rewrite <- TS0, <- join_r. ss. }
+              unfold FwdItem.read_view. s. condtac; cycle 1.
+              { i. eapply sim_mem_read; eauto. rewrite <- TS0, <- join_r. ss. }
+              i. destruct (equiv_dec ts1 ts0); ss. inv e.
+              inv LOCAL. specialize (FWDBANK (ValA.val (sem_expr rmap2 eloc))). inv FWDBANK; [congr|].
+              rewrite FWD in H. inv H. ss. exploit REL.
+              { rewrite <- TS0, <- join_r. ss. }
+              i. des.
+              unfold FwdItem.read_view. ss. 
+              
+              ; s; cycle 1.
+              { rewrite <- TS0, <- join_r. ss. }
+              
+              { rewrite <- TS0, <- join_r. ss. }
+              inv e. 
+
+inv WF2. inv LOCAL0. ss. exploit FWDBANK; eauto. s. i. des.
+              rewrite x. inv LOCAL. apply COH1. 
+                
+
+  FWD : Local.fwdbank lc2 (ValA.val (sem_expr rmap2 eloc)) =
+        Some {| FwdItem.ts := ts1; FwdItem.view := view; FwdItem.ex := ex |}
+                
+              - rewrite <- join_r. ss.
+            }
+              inv MEM. specialize (MEM (S ts0).
+              admit. }
+          * econs 3; ss.
+        + econs; ss.
+          * admit.
+          * admit.
+      }
+      { (* read's post-view > ts. *)
+        admit.
+      }
+      (*       1, 2, 3: eauto. *)
+      (*       econs; eauto. *)
+      (*     * s. econs 2. ss. *)
+      (*   + econs; ss. econs; ss; try by apply LOCAL. *)
+      (*     * apply sim_rmap_add; ss. apply sim_rmap_expr. ss. *)
+      (*     * rewrite bot_join; [|by apply View.order]. destruct lc1. ss. *)
+
+      (*   eexists (ExecUnit.mk _ _ _). esplits; [econs 2; [|econs 1]|]. *)
+      (*   - left. econs; ss. *)
+      (*     assert (ELOC: sem_expr rmap1 eloc = sem_expr rmap2 eloc). *)
+      (*     { eapply sim_rmap_expr; eauto. rewrite <- VCAP, <- join_r. refl. } *)
+      (*     econs; ss; cycle 1. *)
+      (*     + econs 2; eauto. econs. *)
+      (*       4: instantiate (1 := ts0). *)
+      (*       1: instantiate (1 := (sem_expr rmap1 eloc)). *)
+      (*       all: ss. *)
+      (*       all: rewrite ELOC. *)
+      (*       * inv LOCAL0. specialize (COH0 (ValA.val (sem_expr rmap2 eloc))). inv COH0. *)
+      (*         rewrite TS; ss. etrans; eauto. *)
+      (*       * admit. (* hard: coh <= ts0, so no additional messages *) *)
+      (*       * rewrite <- MSG. inv MEM. unfold Memory.read. destruct ts0; ss. *)
+      (*         rewrite ? nth_error_app1; ss. *)
+      (*     + econs 3; ss. *)
+      (*   - econs; ss. econs; ss. *)
+      (*     + admit. (* sim_state *) *)
+      (*     + admit. (* sim_lc *) *)
+      (* } *)
+      (* { (* read from new msg. *) *)
+      (*   admit. *)
+      (* } *)
+    - (* fulfill *)
+      inv STEP.
+      assert (TS0: ts0 <= ts).
+      { inv WRITABLE. inv LOCAL. exploit PROMISES_TS; eauto. }
+      exploit sim_rmap_expr; eauto. i. inv x1. exploit TS.
+      { rewrite <- TS0. inv WRITABLE. etrans; [|by apply Time.lt_le_incl; eauto].
+        s. rewrite <- join_l. eauto.
+      }
+      intro ELOC. clear TS.
+      exploit sim_rmap_expr; eauto. i. inv x1. exploit TS.
+      { rewrite <- TS0. inv WRITABLE. etrans; [|by apply Time.lt_le_incl; eauto].
+        s. rewrite <- join_r, <- join_l. eauto.
+      }
+      intro EVAL. clear TS.
+      eexists (ExecUnit.mk _ _ _). esplits.
+      + econs 1. econs. econs; ss; cycle 1.
+        * econs 3; eauto. econs; eauto; cycle 1.
+          { rewrite <- MSG. apply MEM. ss. }
+          { inv LOCAL. rewrite PROMISES. eauto. }
+          { instantiate (1 := view_ext).
+            instantiate (1 := ord).
+            instantiate (1 := ex0).
+            inv WRITABLE. econs; eauto.
+            - symmetry. eapply sim_view_eq; cycle 1.
+              { etrans; [by apply Time.lt_le_incl; eauto|]. eauto. }
+              s. repeat apply sim_view_join; ss.
+              all: try apply sim_view_ifc.
+              all: try by apply LOCAL.
+              inv LOCAL. inv EXBANK; ss. inv REL. ss.
+            - exploit sim_time_eq.
+              { inv LOCAL. eapply COH0. }
+              { etrans; [by apply Time.lt_le_incl; eauto|]. eauto. }
+              i. congr.
+            - admit. (* exclusive on old message *)
+          }
+        * econs 4; ss.
+      + econs; ss; eauto using sim_rmap_add, sim_val_const.
+        inv LOCAL. econs; ss; i.
+        all: repeat rewrite fun_add_spec.
+        all: repeat apply sim_view_join; ss.
+        * condtac; ss.
+        * condtac; ss. econs. s. splits; ss.
+        * destruct ex0; ss.
+        * congr.
+        * revert FIND. rewrite Promises.unset_o. condtac; ss. eauto.
+    - (* write_failure *)
+      inv STEP. eexists (ExecUnit.mk _ _ _). esplits.
+      + econs 1. econs. econs; ss; cycle 1.
+        * econs 4; eauto. econs; eauto.
+        * econs 4; ss.
+      + econs; ss. econs; ss; eauto using sim_rmap_add, sim_val_const.
+        inv LOCAL. econs; ss.
+    - (* isb *)
+      inv STEP. eexists (ExecUnit.mk _ _ _). esplits.
+      + econs 1. econs. econs; ss; cycle 1.
+        * econs 5; eauto. econs; eauto.
+        * econs 5.
+      + econs; ss. inv LOCAL. econs; eauto using sim_view_join.
+    - (* dmb *)
+      inv STEP. eexists (ExecUnit.mk _ _ _). esplits.
+      + econs 1. econs. econs; ss; cycle 1.
+        * econs 6; eauto. econs; eauto.
+        * econs 5.
+      + econs; ss. inv LOCAL. econs; eauto 10 using sim_view_join, sim_view_ifc.
+    - (* if *)
+      inv LC. eexists (ExecUnit.mk _ _ _). esplits.
+      + econs 1. econs. econs; ss; cycle 1.
+        * econs 1; eauto. econs; eauto.
+        * econs 6; ss.
+      + exploit sim_rmap_expr; eauto. i. inv x1. exploit TS.
+        { rewrite <- VCAP. apply join_r. }
+        intro ELOC. econs; ss.
+        { econs; ss. rewrite ELOC. ss. }
+        econs; ss; try by apply LOCAL.
+        apply sim_view_join; try by apply LOCAL.
+        rewrite x. ss.
+    - (* dowhile *)
+      apply internal_bot_inv in LC. subst.
+      eexists (ExecUnit.mk _ _ _). esplits.
+      + econs 1. econs. econs; ss; cycle 1.
+        * econs 1; eauto. econs; eauto.
+        * econs 7. ss.
+      + econs; ss. econs; ss; try by apply LOCAL.
+        rewrite bot_join; [|by apply View.order]. apply LOCAL.
+  }
+Admitted.
+      
+
 
 Lemma sim_certify
       tid eu1 eu2
